Heap/RemoveEdge.v
@@ -15,23 +15,11 @@ Local Open Scope sets.
 Local Open Scope Z.
 Local Open Scope monad.
 
+
 Fact remove_go_left_edge_fact1: forall (v lc: Z) (V: Z -> Prop),
   Hoare (fun s => Abs s.(heap) V)
         (remove_go_left_edge v lc)
         (fun _ s => Abs s.(heap) V).
-Admitted.
-
-Fact remove_go_left_edge_fact2: forall (v lc: Z),
-  Hoare (fun s => BinaryTree.legal s.(heap))
-        (remove_go_left_edge v lc)
-        (fun _ s => BinaryTree.legal s.(heap)).
-Admitted.
-
-Fact remove_go_left_edge_fact3: forall (v lc: Z),
-  Hoare (fun s => BinaryTree.legal s.(heap))
-        (remove_go_left_edge v lc)
-        (fun _ s => ~ (exists x, BinaryTree.step_l s.(heap) v x) /\ 
-                    ~ (exists x, BinaryTree.step_u s.(heap) lc x)).
 Admitted.
 
 Fact remove_go_right_edge_fact1: forall (v rc: Z) (V: Z -> Prop),
@@ -40,15 +28,60 @@ Fact remove_go_right_edge_fact1: forall (v rc: Z) (V: Z -> Prop),
         (fun _ s => Abs s.(heap) V).
 Admitted.
 
+Fact remove_go_left_edge'_fact1:
+  forall (v: Z) (a: ExistOrEmpty) (V: Z -> Prop),
+    Hoare (fun s => Abs s.(heap) V)
+          (remove_go_left_edge' v a)
+          (fun _ s => Abs s.(heap) V).
+Admitted.
+
+Fact remove_go_right_edge'_fact1:
+  forall (v: Z) (a: ExistOrEmpty) (V: Z -> Prop),
+    Hoare (fun s => Abs s.(heap) V)
+          (remove_go_right_edge' v a)
+          (fun _ s => Abs s.(heap) V).
+Admitted.
+
+
+
+
+Fact remove_go_left_edge_fact2: forall (v lc: Z),
+  Hoare (fun s => BinaryTree.legal s.(heap))
+        (remove_go_left_edge v lc)
+        (fun _ s => BinaryTree.legal s.(heap) /\ 
+                    ~ (exists x, BinaryTree.step_l s.(heap) v x) /\ 
+                    ~ (exists x, BinaryTree.step_u s.(heap) lc x)).
+Admitted.
+
 Fact remove_go_right_edge_fact2: forall (v rc: Z),
   Hoare (fun s => BinaryTree.legal s.(heap))
         (remove_go_right_edge v rc)
-        (fun _ s => BinaryTree.legal s.(heap)).
-Admitted.
-
-Fact remove_go_right_edge_fact3: forall (v rc: Z),
-  Hoare (fun s => BinaryTree.legal s.(heap))
-        (remove_go_right_edge v rc)
-        (fun _ s => ~ (exists x, BinaryTree.step_r s.(heap) v x) /\ 
+        (fun _ s => BinaryTree.legal s.(heap) /\ 
+                    ~ (exists x, BinaryTree.step_r s.(heap) v x) /\ 
                     ~ (exists x, BinaryTree.step_u s.(heap) rc x)).
 Admitted.
+
+Fact remove_go_left_edge'_fact2:
+  forall (v: Z) (a: ExistOrEmpty),
+    Hoare (fun s => BinaryTree.legal s.(heap))
+          (remove_go_left_edge' v a)
+          (fun _ s => BinaryTree.legal s.(heap) /\ 
+                      ~ (exists x, BinaryTree.step_l s.(heap) v x) /\
+                      match a with
+                      | by_exist lc => ~ (exists x, BinaryTree.step_u s.(heap) lc x)
+                      | by_empty => True
+                      end).
+Admitted.
+
+Fact remove_go_right_edge'_fact2:
+  forall (v: Z) (a: ExistOrEmpty),
+    Hoare (fun s => BinaryTree.legal s.(heap))
+          (remove_go_right_edge' v a)
+          (fun _ s => BinaryTree.legal s.(heap) /\ 
+                      ~ (exists x, BinaryTree.step_r s.(heap) v x) /\
+                      match a with
+                      | by_exist rc => ~ (exists x, BinaryTree.step_u s.(heap) rc x)
+                      | by_empty => True
+                      end).
+Admitted.
+
