Heap/Swapvu.v
@@ -1,0 +1,129 @@
+Require Import Coq.Lists.List.
+Require Import Coq.ZArith.ZArith.
+Require Import Coq.Classes.RelationClasses.
+Require Import PL.Monad.
+Require Import PL.Monad2.
+Require Import SetsClass.
+Require Import HEAP.Defs.
+Require Import Classical.
+Require Import Coq.Setoids.Setoid.
+Require Import Coq.micromega.Psatz.
+Require Import HEAP.AddEdge.
+Require Import HEAP.RemoveEdge.
+Import SetsNotation
+       StateRelMonad
+       StateRelMonadOp
+       StateRelMonadHoare
+       MonadNotation
+       Monad.
+Local Open Scope sets.
+Local Open Scope Z.
+Local Open Scope monad.
+
+Fact get_lc_fact: forall (v: Z) P, 
+  Hoare P (get_lc v) (fun lc s => P s /\ BinaryTree.step_l s.(heap) v lc).
+Proof.
+  intros.
+  unfold Hoare, get_lc; sets_unfold.
+  intros. destruct H0.
+  split.
+  - rewrite H1. tauto.
+  - rewrite H1. tauto.
+Qed.
+
+Fact get_lc'_fact: forall (v: Z) P, 
+  Hoare P (get_lc' v)
+    (fun a s => P s /\ match a with
+                      | by_exist lc => BinaryTree.step_l s.(heap) v lc
+                      | by_empty => ~ (exists x, BinaryTree.step_l s.(heap) v x)
+                      end).
+Proof.
+  intros.
+  unfold get_lc'.
+  apply Hoare_choice.
+  + apply Hoare_test_bind.
+    apply Hoare_ret'.
+    tauto.
+  + eapply Hoare_bind; [apply get_lc_fact| cbv beta].
+    intros lc.
+    apply Hoare_ret'.
+    tauto.
+Qed.
+
+
+Fact get_rc'_fact: forall (v: Z) P, 
+  Hoare P (get_rc' v)
+    (fun a s => P s /\ match a with
+                      | by_exist rc => BinaryTree.step_l s.(heap) v rc
+                      | by_empty => True
+                      end).
+Admitted.
+
+Fact get_dir_fact: forall (fa v: Z) P, 
+  Hoare P (get_dir fa v)
+    (fun dir s => P s /\
+      (
+        (dir = 0 /\ BinaryTree.step_l s.(heap) fa v) \/
+        (dir = 1 /\ BinaryTree.step_r s.(heap) fa v))
+      ).
+Admitted.
+
+Fact swap_v_fa_fact1: forall (v fa: Z) (V: Z -> Prop), 
+  Hoare
+    (fun s => v < fa /\
+              ((s.(heap)).(vvalid) v /\
+                Abs s.(heap) V /\
+                BinaryTree.legal s.(heap) /\
+                (Heap s.(heap) \/ Heap_broken_up s.(heap) v)) /\
+              BinaryTree.step_u s.(heap) v fa)
+    (swap_v_u v fa)
+    (fun _ s => (s.(heap)).(vvalid) v /\
+                Abs s.(heap) V /\
+                BinaryTree.legal s.(heap) /\
+                (Heap s.(heap) \/ Heap_broken_up s.(heap) v)).
+Admitted.
+
+Fact swap_v_fa_fact2: forall (v fa: Z), 
+  Hoare
+    (fun s => v < fa /\
+              ((s.(heap)).(vvalid) v /\
+                BinaryTree.legal s.(heap) /\
+                is_complete_or_full_bintree s.(heap)) /\
+              BinaryTree.step_u s.(heap) v fa)
+    (swap_v_u v fa)
+    (fun _ s => (s.(heap)).(vvalid) v /\
+                BinaryTree.legal s.(heap) /\
+                is_complete_or_full_bintree s.(heap)).
+Admitted.
+
+Fact swap_v_fa_fact3: forall (v fa: Z) (V: Z -> Prop), 
+  Hoare
+    (fun s => Abs s.(heap) V)
+    (swap_v_u v fa)
+    (fun _ s => Abs s.(heap) V).
+Admitted.
+
+Fact swap_v_fa_fact4: forall (v fa: Z), 
+  Hoare
+    (fun s => BinaryTree.legal s.(heap) /\
+              BinaryTree.step_u s.(heap) v fa)
+    (swap_v_u v fa)
+    (fun _ s => BinaryTree.legal s.(heap)).
+Proof.
+  intros.
+  unfold swap_v_u.
+  eapply Hoare_bind; [apply get_lc'_fact| cbv beta; intros lc_v].
+  eapply Hoare_bind; [apply get_rc'_fact| cbv beta; intros rc_v].
+  eapply Hoare_bind; [apply get_lc'_fact| cbv beta; intros lc_fa].
+  eapply Hoare_bind; [apply get_rc'_fact| cbv beta; intros rc_fa].
+  eapply Hoare_bind; [apply get_dir_fact| cbv beta; intros dir_fa_v].
+Admitted.
+  (* eapply Hoare_bind.
+  - apply (remove_go_left_edge'_fact2 v lc_v). *)
+
+  
+  
+
+
+  
+  
